src/opt/UnusedLoad.v
@@ -83,8 +83,8 @@ Proof.
   { exploit unused_read; eauto. i. des.
     exploit sim_local_read; eauto; try refl. i. des.
     esplits.
-    - econs 2; eauto. econs. econs 2. econs 2; eauto.
-      + econs. econs.
+    - econs 2; eauto. econs.
+      + econs. econs 2. econs 2; eauto. econs. econs.
       + eauto.
     - auto.
     - auto.
