src/prop/ReorderPromises.v
@@ -18,16 +18,15 @@ Require Import TView.
 Require Import Thread.
 Require Import Configuration.
 
-Require Import PFStep.
 Require Import PromiseConsistent.
 Require Import ReorderPromiseSame.
 
 Set Implicit Arguments.
 
 
-Lemma rtc_step_evt_promise_consistent
+Lemma rtc_all_step_promise_consistent
       lang th1 th2
-      (STEP: rtc (@step_evt lang) th1 th2)
+      (STEP: rtc (@Thread.all_step lang) th1 th2)
       (CONS: promise_consistent th2.(Thread.local))
       (WF1: Local.wf th1.(Thread.local) th1.(Thread.memory))
       (SC1: Memory.closed_timemap th1.(Thread.sc) th1.(Thread.memory))
@@ -35,81 +34,80 @@ Lemma rtc_step_evt_promise_consistent
   promise_consistent th1.(Thread.local).
 Proof.
   revert_until STEP. induction STEP; auto. i.
-  inv H. exploit Thread.step_future; eauto. i. des.
+  inv H. inv USTEP. exploit Thread.step_future; eauto. i. des.
   eapply step_promise_consistent; eauto.
 Qed.
 
 Lemma steps_pf_steps_aux
       lang
       n e1 e3
-      (STEPS: rtcn (@step_evt lang) n e1 e3)
+      (STEPS: rtcn (@Thread.all_step lang) n e1 e3)
       (CONS: promise_consistent e3.(Thread.local))
       (WF1: Local.wf e1.(Thread.local) e1.(Thread.memory))
       (SC1: Memory.closed_timemap e1.(Thread.sc) e1.(Thread.memory))
       (MEM1: Memory.closed e1.(Thread.memory)):
   exists n' e2,
     <<N: n' <= n>> /\
-    <<STEPS1: rtcn (@pf_step_evt lang) n' e1 e2>> /\
-    <<STEPS2: rtc (@nonpf_step_evt lang) e2 e3>>.
+    <<STEPS1: rtcn (union (Thread.step true)) n' e1 e2>> /\
+    <<STEPS2: rtc (union (Thread.step false)) e2 e3>>.
 Proof.
   revert_until n. induction n using strong_induction; i.
   inv STEPS.
   { esplits; eauto. }
-  inv A12. exploit pf_step_dec; eauto. i. des.
-  { exploit pf_step_future; eauto. i. des.
+  inv A12. inv USTEP. exploit Thread.step_future; eauto. i. des.
+  destruct pf.
+  { exploit Thread.step_future; eauto. i. des.
     exploit IH; eauto. i. des.
     esplits; cycle 1.
-    + econs 2; eauto. econs; eauto.
+    + econs 2; eauto.
     + auto.
     + omega.
   }
-  exploit nonpf_step_future; eauto. i. des.
   exploit IH; try exact A23; try refl; eauto. i. des.
   assert (CONS2: promise_consistent (Thread.local e2)).
   { exploit rtcn_rtc; try exact A0; eauto. i.
-    exploit rtc_implies; (try by apply pf_step_evt_step_evt); eauto. i.
-    exploit rtc_step_evt_future; eauto. i. des.
-    eapply rtc_step_evt_promise_consistent; try exact CONS; eauto.
+    exploit rtc_implies; [|exact x0|i].
+    { apply union_mon. apply Thread.allpf. }
+    exploit Thread.rtc_all_step_future; eauto. i. des.
+    eapply rtc_all_step_promise_consistent; try exact CONS; eauto.
     eapply rtc_implies; try exact STEPS2; eauto.
-    apply nonpf_step_evt_step_evt.
+    apply union_mon. apply Thread.allpf.
   }
   inv STEPS1.
   { esplits; cycle 1.
     - eauto.
-    - econs; eauto. econs. eauto.
+    - econs; eauto.
     - omega.
   }
-  inversion A12. exploit pf_step_future; eauto. i. des.
+  inversion A12. exploit Thread.step_future; eauto. i. des.
   exploit reorder_nonpf_pf; eauto.
   { exploit rtcn_rtc; try exact A0; eauto. i.
-    eapply rtc_step_evt_promise_consistent; try exact CONS; eauto.
+    eapply rtc_all_step_promise_consistent; try exact CONS; eauto.
     etrans.
-    - eapply rtc_implies; try exact x1; eauto.
-      apply pf_step_evt_step_evt.
-    - eapply rtc_implies; try exact STEPS2; eauto.
-      apply nonpf_step_evt_step_evt.
+    - eapply rtc_implies; [|exact x0]. apply union_mon. apply Thread.allpf.
+    - eapply rtc_implies; [|exact STEPS2]. apply union_mon. apply Thread.allpf.
   }
   i. des.
-  - assert (STEPS: rtcn (step_evt (lang:=lang)) (S n) e1 e2).
+  - assert (STEPS: rtcn (@Thread.all_step lang) (S n) e1 e2).
     { econs 2.
-      - econs. eauto.
-      - eapply rtcn_imply; try exact A0. apply pf_step_evt_step_evt.
+      - econs. econs. eauto.
+      - eapply rtcn_imply; [|exact A0]. apply union_mon. apply Thread.allpf.
     }
     exploit IH; try exact STEPS; eauto.
     { omega. }
     i. des. esplits; cycle 1; eauto.
     + etrans; eauto.
     + omega.
-  - assert (STEPS: rtcn (step_evt (lang:=lang)) (S n) th1' e2).
+  - assert (STEPS: rtcn (@Thread.all_step lang) (S n) th1' e2).
     { econs 2.
       - econs. econs 1. eauto.
-      - eapply rtcn_imply; try exact A0. apply pf_step_evt_step_evt.
+      - eapply rtcn_imply; [|exact A0]. apply union_mon. apply Thread.allpf.
     }
-    exploit pf_step_future; eauto. i. des.
+    exploit Thread.step_future; eauto. i. des.
     exploit IH; try exact STEPS; eauto.
     { omega. }
     i. des. esplits; cycle 1.
-    + econs 2; eauto. econs. eauto.
+    + econs 2; eauto.
     + etrans; eauto.
     + omega.
 Qed.
@@ -117,14 +115,14 @@ Qed.
 Lemma steps_pf_steps
       lang
       e1 e3
-      (STEPS: rtc (@step_evt lang) e1 e3)
+      (STEPS: rtc (@Thread.all_step lang) e1 e3)
       (CONS: promise_consistent e3.(Thread.local))
       (WF1: Local.wf e1.(Thread.local) e1.(Thread.memory))
       (SC1: Memory.closed_timemap e1.(Thread.sc) e1.(Thread.memory))
       (MEM1: Memory.closed e1.(Thread.memory)):
   exists e2,
-    <<STEPS1: rtc (@pf_step_evt lang) e1 e2>> /\
-    <<STEPS2: rtc (@nonpf_step_evt lang) e2 e3>>.
+    <<STEPS1: rtc (union (Thread.step true)) e1 e2>> /\
+    <<STEPS2: rtc (union (Thread.step false)) e2 e3>>.
 Proof.
   apply rtc_rtcn in STEPS. des.
   exploit steps_pf_steps_aux; eauto. i. des.
@@ -141,64 +139,64 @@ Lemma tau_steps_pf_tau_steps_aux
       (MEM1: Memory.closed e1.(Thread.memory)):
   exists n' e2,
     <<N: n' <= n>> /\
-    <<STEPS1: rtcn (@tau_pf_step lang) n' e1 e2>> /\
-    <<STEPS2: rtc (@nonpf_step_evt lang) e2 e3>>.
+    <<STEPS1: rtcn (tau (Thread.step true)) n' e1 e2>> /\
+    <<STEPS2: rtc (tau (Thread.step false)) e2 e3>>.
 Proof.
   revert_until n. induction n using strong_induction; i.
   inv STEPS.
   { esplits; eauto. }
-  inv A12. exploit pf_step_dec; eauto. i. des.
-  { exploit pf_step_future; eauto. i. des.
+  inv A12. inv TSTEP. exploit Thread.step_future; eauto. i. des.
+  destruct pf.
+  { exploit Thread.step_future; eauto. i. des.
     exploit IH; eauto. i. des.
     esplits; cycle 1.
-    + econs 2; eauto. econs; eauto.
+    + econs 2; eauto.
     + auto.
     + omega.
   }
-  exploit nonpf_step_future; eauto. i. des.
   exploit IH; try exact A23; try refl; eauto. i. des.
   assert (CONS2: promise_consistent (Thread.local e2)).
   { exploit rtcn_rtc; try exact A0; eauto. i.
-    exploit rtc_implies; (try by apply tau_pf_step_pf_step_evt); eauto. i.
-    exploit rtc_implies; (try by apply pf_step_evt_step_evt); eauto. i.
-    exploit rtc_step_evt_future; eauto. i. des.
-    eapply rtc_step_evt_promise_consistent; try exact CONS; eauto.
+    exploit rtc_implies; [|exact x0|i].
+    { apply tau_mon. apply Thread.allpf. }
+    exploit Thread.rtc_tau_step_future; eauto. i. des.
+    eapply rtc_all_step_promise_consistent; try exact CONS; eauto.
     eapply rtc_implies; try exact STEPS2; eauto.
-    apply nonpf_step_evt_step_evt.
+    i. apply tau_union. eapply tau_mon; [|eauto]. apply Thread.allpf.
   }
   inv STEPS1.
   { esplits; cycle 1.
     - eauto.
-    - econs; eauto. econs. eauto.
+    - econs; eauto.
     - omega.
   }
-  inversion A12. exploit pf_step_future; eauto. i. des.
+  inversion A12. exploit Thread.step_future; eauto. i. des.
   exploit reorder_nonpf_pf; eauto.
   { exploit rtcn_rtc; try exact A0; eauto. i.
-    eapply rtc_step_evt_promise_consistent; try exact CONS; eauto.
+    eapply rtc_all_step_promise_consistent; try exact CONS; eauto.
     etrans.
-    - eapply rtc_implies; try exact x1; eauto.
-      i. apply pf_step_evt_step_evt. apply tau_pf_step_pf_step_evt. ss.
-    - eapply rtc_implies; try exact STEPS2; eauto.
-      apply nonpf_step_evt_step_evt.
+    - eapply rtc_implies; [|exact x0]. i. apply tau_union. eapply tau_mon; [|eauto]. apply Thread.allpf.
+    - eapply rtc_implies; [|exact STEPS2]. i. apply tau_union. eapply tau_mon; [|eauto]. apply Thread.allpf.
   }
   i. des.
-  - assert (STEPS: rtcn (Thread.tau_step (lang:=lang)) (S n) e1 e2).
+  - assert (STEPS: rtcn (@Thread.tau_step lang) (S n) e1 e2).
     { econs 2.
-      - econs; eauto. etrans; eauto.
-      - eapply rtcn_imply; try exact A0. apply tau_pf_step_tau_step.
+      - econs. econs; eauto. etrans; eauto.
+      - eapply rtcn_imply; [|exact A0]. apply tau_mon. apply Thread.allpf.
     }
     exploit IH; try exact STEPS; eauto.
     { omega. }
     i. des. esplits; cycle 1; eauto.
     + etrans; eauto.
     + omega.
-  - assert (STEPS: rtcn (Thread.tau_step (lang:=lang)) (S n) th1' e2).
+  - assert (STEPS: rtcn (@Thread.tau_step lang) (S n) th1' e2).
     { econs 2.
-      - econs. econs; eauto. by inv STEP2.
-      - eapply rtcn_imply; try exact A0. apply tau_pf_step_tau_step.
+      - econs.
+        + econs. econs 1. eauto.
+        + inv STEP2. ss.
+      - eapply rtcn_imply; [|exact A0]. apply tau_mon. apply Thread.allpf.
     }
-    exploit pf_step_future; eauto. i. des.
+    exploit Thread.step_future; eauto. i. des.
     exploit IH; try exact STEPS; eauto.
     { omega. }
     i. des. esplits; cycle 1.
@@ -216,21 +214,21 @@ Lemma tau_steps_pf_tau_steps
       (SC1: Memory.closed_timemap e1.(Thread.sc) e1.(Thread.memory))
       (MEM1: Memory.closed e1.(Thread.memory)):
   exists e2,
-    <<STEPS1: rtc (@tau_pf_step lang) e1 e2>> /\
-    <<STEPS2: rtc (@nonpf_step_evt lang) e2 e3>>.
+    <<STEPS1: rtc (tau (Thread.step true)) e1 e2>> /\
+    <<STEPS2: rtc (tau (Thread.step false)) e2 e3>>.
 Proof.
   apply rtc_rtcn in STEPS. des.
   exploit tau_steps_pf_tau_steps_aux; eauto. i. des.
   exploit rtcn_rtc; eauto.
 Qed.
 
-Lemma nonpf_step_evt_bot
+Lemma union_step_nonpf_bot
       lang e1 e2
-      (STEP: @nonpf_step_evt lang e1 e2)
+      (STEP: union (@Thread.step lang false) e1 e2)
       (PROMISE: e2.(Thread.local).(Local.promises) = Memory.bot):
   False.
 Proof.
-  inv STEP. inv STEP0. inv LOCAL. ss. subst. inv PROMISE0.
+  inv STEP. inv USTEP. inv STEP. inv LOCAL. ss. subst. inv PROMISE0.
   - exploit (@Memory.add_o Memory.bot lc1.(Local.promises) loc from to val released loc to)
     ; try exact PROMISES; eauto. condtac; ss; [|des; congr].
     rewrite Memory.bot_get. congr.
@@ -242,12 +240,12 @@ Proof.
     rewrite Memory.bot_get. congr.
 Qed.
 
-Lemma rtc_nonpf_step_evt_bot
+Lemma rtc_union_step_nonpf_bot
       lang e1 e2
-      (STEPS: rtc (@nonpf_step_evt lang) e1 e2)
+      (STEP: rtc (union (@Thread.step lang false)) e1 e2)
       (PROMISE: e2.(Thread.local).(Local.promises) = Memory.bot):
   e1 = e2.
 Proof.
   exploit rtc_tail; eauto. i. des; ss.
-  exfalso. eapply nonpf_step_evt_bot; eauto.
+  exfalso. eapply union_step_nonpf_bot; eauto.
 Qed.
